Lambda_Calcul.v: Added examples

Lambda_Calcul.v
@@ -6,7 +6,7 @@ Inductive lambda_term : Set :=
 | abstraction : lambda_term -> lambda_term
 | application : lambda_term -> lambda_term -> lambda_term.
 
-Fixpoint br_vieux (n : nat) (t : lambda_term) (u : lambda_term) : lambda_term :=
+Fixpoint br_fix (n : nat) (t u : lambda_term) : lambda_term :=
   match t with
   (* variable libre *)
   | variable x => variable x
@@ -17,15 +17,31 @@ Fixpoint br_vieux (n : nat) (t : lambda_term) (u : lambda_term) : lambda_term :=
        | _ => reference m
        end
   (* on passe un lambda donc on incrémente l'indice *)
-  | abstraction x => br_vieux (n + 1) x u
+  | abstraction x => br_fix (n + 1) x u
   (* on passe au contexte *)
-  | (application t1 t2) => application (br_vieux n t1 u) (br_vieux n t2 u)
+  | (application t1 t2) => application (br_fix n t1 u) (br_fix n t2 u)
   end.
+
+Fixpoint beta_reduction_fix (t u : lambda_term) : option lambda_term :=
+    match t with
+    | abstraction x => Some (br_fix 0 x u)
+    | variable _ => None
+    | reference _ => None
+    | application _ _ => None
+    end.
+
+Fixpoint redex_fixpoint (t u : lambda_term) : lambda_term :=
+	match t with
+    | abstraction x => br_fix 0 x u
+    | variable _ => t
+    | reference _ => t
+    | application _ _ => t
+    end.
 
 Notation "'var' t" := (variable t) (at level 80, right associativity).
 Notation "'ref' t" := (reference t) (at level 85, right associativity).
 Notation "'λ' t" := (abstraction t) (at level 99, right associativity).
-Notation "t 'app' u" := (application t u) (at level 79, left associativity).
+Notation "'app'" := application (at level 79).
 
 Inductive br : nat -> lambda_term -> lambda_term -> lambda_term -> Prop :=
 | br_variable : forall (n x : nat) (u : lambda_term),
@@ -35,32 +51,86 @@ Inductive br : nat -> lambda_term -> lambda_term -> lambda_term -> Prop :=
 | br_reference_2 : forall (n m : nat) (u : lambda_term),
 	n <> m -> br n (ref m) u (ref m)
 | br_abstraction : forall (n : nat) (t t' u : lambda_term),
-	br (S n) t u t' -> (br n (λ t) u t')
+	br (S n) t u t' -> br n (λ t) u t'
 | br_application : forall (n : nat) (t1 t2 t1' t2' u : lambda_term),
-	br n t1 u t1' -> br n t2 u t2' -> br n (t1 app t2) u (t1' app t2').
+	br n t1 u t1' -> br n t2 u t2' -> br n (app t1 t2) u (app t1' t2').
 
 Inductive beta_reduction : lambda_term -> lambda_term -> Prop :=
 | Beta_redex : forall (t t' u : lambda_term),
-  br 0 t u t' -> beta_reduction ((λ t) app u) t'
+  br 0 t u t' -> beta_reduction (app (λ t) u) t'.
+
+Lemma correction_br : forall (n : nat) (l u : lambda_term), br n l u (br_fix n l u).
+Proof.
+induction n; intros; elim l; intros.
+apply br_variable.
+induction n. apply br_reference. apply br_reference_2; auto.
+apply br_abstraction.
+Admitted.
+
+Inductive beta_ref_trans : lambda_term -> lambda_term -> Prop :=
+| Beta_redex_ref_trans : forall (t u : lambda_term),
+	beta_reduction t u -> beta_ref_trans t u
 | Beta_ref : forall (t : lambda_term),
-	beta_reduction t t
+	beta_ref_trans t t
 | Beta_trans : forall (u t v : lambda_term),
-	beta_reduction t u -> beta_reduction u v -> beta_reduction t v
+	beta_ref_trans t u -> beta_ref_trans u v -> beta_ref_trans t v.
+
+Inductive beta_sym : lambda_term -> lambda_term -> Prop :=
+| Beta_redex_sym : forall (t u : lambda_term),
+	beta_ref_trans t u -> beta_sym t u
 | Beta_sym : forall (v t u : lambda_term),
-	beta_reduction t v -> beta_reduction u v -> beta_reduction t u.
+	beta_sym t v -> beta_sym u v -> beta_sym t u.
 
-Definition id := λ ref 0. (* x -> x *)
+Notation "t '->β' u" := (beta_reduction t u) (at level 86, no associativity).
+Notation "t '->*β' u" := (beta_ref_trans t u) (at level 87, no associativity).
+Notation "t '=β' u" := (beta_sym t u) (at level 88, no associativity).
 
-Goal forall t : lambda_term, beta_reduction (id app t) t.
+Definition id := (λ (ref 0)). (* x -> x *)
+Definition vrai := (λ (λ (ref 1))). (* x,y -> x *)
+Definition faux := (λ (λ (ref 0))). (* x,y -> y *)
+Definition ifthenelse := (λ (λ (λ (app (app (ref 2) (ref 1))) (ref 0)))).
+Definition x := (var 0).
+Definition y := (var 1).
+
+Lemma identity : forall t : lambda_term, app id t ->β t.
 Proof.
 intros.
 apply Beta_redex.
 apply br_reference.
 Qed.
 
-Definition Y := λ (λ ((ref 1) app ((ref 0) app (ref 0))) app ((ref 1) app ((ref 0) app (ref 0)))).
-Lemma fixed_point : forall t : lambda_term, beta_reduction (Y app t) (t app (Y app t)).
+Lemma vrai_id : forall t : lambda_term, app vrai t ->β t.
+Proof.
+intro.
+apply Beta_redex.
+apply br_abstraction.
+apply br_reference.
+Qed.
+
+Goal forall t : lambda_term, (app id t) =β (app vrai t).
 Proof.
 intros.
-apply (Beta_trans (λ (t app ((ref 0) app (ref 0))) app (t app ((ref 0) app (ref 0))))).
-apply Beta_redex. apply br_abstraction.
+apply (Beta_sym t); apply Beta_redex_sym; apply Beta_redex_ref_trans. apply identity. apply vrai_id.
+Qed.
+
+Goal app ifthenelse vrai ->β app (app vrai (ref 1)) (ref 0).
+Proof.
+apply Beta_redex.
+apply br_abstraction.
+apply br_abstraction.
+apply br_application.
+apply br_application.
+apply br_reference.
+apply br_reference_2; auto.
+apply br_reference_2; auto.
+Qed.
+
+Goal app (λ app vrai (ref 1)) (ref 0) ->β (app ((ref 1)) (ref 1)).
+Proof.
+apply Beta_redex.
+apply br_application.
+apply br_abstraction.
+apply br_abstraction.
+apply br_reference_2; auto.
+apply br_reference_2; auto.
+Qed.
